% \iffalse
\documentclass[journal,12pt,twocolumn]{article}
\usepackage{amsmath,amssymb,amsfonts,amsthm}
\usepackage{txfonts}
\usepackage{tkz-euclide} 
\usepackage{listings}
\usepackage{gvv}       
\usepackage[latin1]{inputenc}   
\usepackage{array}  

\begin{document}

\bibliographystyle{IEEEtran}

\vspace{3cm}

\title{}
\author{EE23BTECH11217 - Prajwal M$^{*}$
}
\maketitle
\newpage
\bigskip

\renewcommand{\thefigure}{\theenumi}
\renewcommand{\thetable}{\theenumi}

\section*{Exercise 9.5}
\noindent25) \hspace{2pt} \textbf{Find the sum of the following series up to n terms and obtain the Z-transform:}
$$ 
\ldots + 0 + \frac{1^3}{1} + \frac{1^3 + 2^3}{1 + 3} + \frac{1^3 + 2^3 + 3^3}{1 + 3 + 5} + \ldots$$

\noindent Solution: 

\begin{table}[h]
    \centering
    \input{tables/table}
    \caption{Parameters}
    \label{tab: 11.9.5.25.1}
\end{table}

\begin{align}
    x\brak{n} & = \frac{\sum_{i=0}^{n} \brak{i+1}^{3}}{\sum_{i=0}^{n} \brak{2i+1}} u\brak{n}  \\
    & = \frac{x_1\brak{n}}{x_2\brak{n}}u\brak{n} \label{eq: 9.5.25.1}
\end{align}
\begin{align}
    x_1\brak{n} & = \sum_{i=0}^{n} \brak{i+1}^{3}\\
    & = \brak{n+1}^{3} * u\brak{n}\\
    x_1\brak{n} & \system{Z} X_1\brak{z}\\
    X_1\brak{z} & = \brak{\frac{1 + 4z^{-1} + z^{-2}}{\brak{1-z^{-1}}^4}} \brak{\frac{1}{1-z^{-1}}}\\
    & = \frac{1}{(1 - z^{-1})^5} + \frac{4 z^{-1}}{(1 - z^{-1})^5} + \frac{z^{-2}}{(1 - z^{-1})^5}\\
    x_1\brak{n} & = \frac{\brak{n + 4} \brak{n + 3} \brak{n + 2} \brak{n + 1}}{24}u\brak{n+4}\\
    & + \frac{\brak{n + 3} \brak{n + 2} \brak{n + 1} n}{6}u\brak{n+3}\notag\\
    & + \frac{\brak{n + 2} \brak{n + 1} n \brak{n - 1}}{24}u\brak{n+2}\notag\\
    & = \frac{\brak{n+2}^2\brak{n+1}^2}{4}u\brak{n}
\end{align}
\begin{align}
    x_2\brak{n} & = \sum_{i=0}^{n} \brak{2i+1}\\
    & = \brak{2n+1} * u\brak{n}\\
    x_2\brak{n} & \system{Z} X_2\brak{z}\\
    X_2\brak{z} & = \brak{\frac{1 + z^{-1}}{\brak{1-z^{-1}}^2}} \brak{\frac{1}{1-z^{-1}}}\\
    & = \frac{1}{(1 - z^{-1})^3} + \frac{z^{-1}}{(1 - z^{-1})^3}\\
    x_2\brak{n} & = \frac{\brak{n + 2} \brak{n + 1}}{2}u\brak{n+2}\\
    & + \frac{\brak{n + 1} \brak{n} }{2}u\brak{n+1}\notag\\
    & = \brak{n+1}^2u\brak{n}\\
    \notag \text{using \eqref{9.5.25.1}, } \\
    x\brak{n} & = \frac{\brak{n+2}^2}{4} u\brak{n}\label{eq: 9.5.25.2}
\end{align}

\begin{align}
    s\brak{n} & = \sum_{r=-\infty}^{n} x\brak{r}\\
    \notag \text{using \eqref{9.5.25.2}, } \\
    s\brak{n} & = \sum_{r=-\infty}^{n} \frac{\brak{r+2}^{2}}{4} u\brak{r} \\
    & = \frac{\brak{n+2}^2}{4} * u\brak{n}\\
    s\brak{n} & \system{Z} S\brak{z}\\
    S\brak{z} & = \brak{\frac{4 -3z^{-1} + z^{-2}}{4\brak{1-z^{-1}}^3}} \brak{\frac{1}{1-z^{-1}}}\\
    & = \frac{1}{(1 - z^{-1})^4} - \frac{3z^{-1}}{4(1 - z^{-1})^4} \\
    & + \frac{z^{-2}}{4(1 - z^{-1})^4}\\
    s\brak{n} & = \frac{\brak{n + 3} \brak{n + 2}\brak{n+1}}{6}u\brak{n+3}\\
    & - \frac{\brak{n + 2} \brak{n + 1}\brak{n}}{8}u\brak{n+2}\notag\\
    & + \frac{\brak{n + 1} \brak{n}\brak{n-1}}{24}u\brak{n+1}\\
    & = \brak{1 + \frac{37n}{24} + \frac{5n^2}{8} + \frac{n^3}{12}} u\brak{n} 
\end{align}

\begin{figure}[h]
   \centering
   \includegraphics[width=1\columnwidth]{figs/plot.png}
   \caption{Plot of x(n) vs n}
   \label {fig: 11.9.5.25.1}
\end{figure}


\end{document}

