
\documentclass[journal,12pt,twocolumn]{IEEEtran}
\usepackage{amsmath,amssymb,amsfonts,amsthm}
\usepackage{txfonts}
\usepackage{tkz-euclide} 
\usepackage{listings}
\usepackage{gvv}       
\usepackage[latin1]{inputenc}   
\usepackage{array}  

\begin{document}

\bibliographystyle{IEEEtran}

\vspace{3cm}

\title{}
\author{EE23BTECH11217 - Prajwal M$^{*}$
}
\maketitle
\newpage
\bigskip

\renewcommand{\thefigure}{\theenumi}
\renewcommand{\thetable}{\theenumi}

\section*{Exercise 9.1}

\noindent \textbf{12) \hspace{2pt}Write the first five terms of each of the sequences and obtain the corresponding series}
$x(1) = -1$, $x(n) = \dfrac{x({n-1})}{n}$, $n \geq 2$\\

\noindent Solution: 

\noindent Given: $x(1) = -1$, $x(n) = \dfrac{x({n-1})}{n}$, $n \geq 2$. \\

First five terms of the sequence:

\begin{align*}
x(1) & = -1 \\
x(2) & = \frac{x(1)}{2} = -\frac{1}{2} \\
x(3) & = \frac{x(2)}{3} = -\frac{1}{2 \cdot 3} = -\frac{1}{6}\\
x(4) & = \frac{x(3)}{4} = -\frac{1}{2 \cdot 3 \cdot 4} = -\frac{1}{24}\\
x(5) & = \frac{x(4)}{5} = -\frac{1}{2 \cdot 3 \cdot 4 \cdot 5} = -\frac{1}{120}
\end{align*} \\

So the first five terms of the series are: 
$$-1 , -\frac{1}{2}, -\frac{1}{6}, -\frac{1}{24},  -\frac{1}{120}$$ \\

The corresponding series:
\begin{align*}
    \sum_{n=1}^{\infty} x(n) & = x(1) + x(2) + x(3) + x(4) + x(5) + \ldots \\
    & = -1 + \left(-\frac{1}{2}\right) + \left(-\frac{1}{6}\right) + \left(-\frac{1}{24}\right) + \ldots \\ 
\end{align*}

The nth term of the series is, 
\begin{align*}
    x(n) & = \frac{-1}{n!} (u(n))
\end{align*} 

The Z-transform of $ x(n) $ is given by:
$$x(n) \ztransform F(z)$$

\begin{align*}
    F(z) & = \sum_{n=-\infty}^{\infty} x(n) \cdot z^{-n} \\
    & = \sum_{n=-\infty}^{\infty} \frac{-1}{n!}\cdot u(n) \cdot z^{-n} \\
    & = \sum_{n=1}^{\infty} \frac{-1}{n!} \cdot z^{-n} \\
    & = - (e^{z^{-1}} - 1) \\
    & = 1 - e^{z^{-1}}  
\end{align*}

So, the Z-transform of the given series is 
$ 1 - e^{z^{-1}} $.

\end{document}
